Even better sexact

MPL/ProofMode/Tactics/Exact.lean
@@ -10,7 +10,7 @@ theorem Exact.assumption {σs : List Type} {P P' A : SPred σs}
 theorem Exact.from_tautology {σs : List Type} {P T : SPred σs} (htaut : ⊢ₛ T) : P ⊢ₛ T :=
   SPred.true_intro.trans htaut
 
-def _root_.MPL.ProofMode.SGoal.exact (goal : SGoal) (hyp : TSyntax `ident) : OptionT MetaM Expr := do
+def _root_.MPL.ProofMode.SGoal.exact (goal : SGoal) (hyp : TSyntax `term) : OptionT MetaM Expr := do
   let some focusRes := goal.focusHyp hyp.raw.getId | failure
   OptionT.mk do
   let proof := mkApp5 (mkConst ``Exact.assumption) goal.σs goal.hyps focusRes.restHyps goal.target focusRes.proof
@@ -18,22 +18,21 @@ def _root_.MPL.ProofMode.SGoal.exact (goal : SGoal) (hyp : TSyntax `ident) : Opt
     throwError "sexact tactic failed, hypothesis {hyp} is not definitionally equal to {goal.target}"
   return proof
 
-def _root_.MPL.ProofMode.SGoal.exactPure (goal : SGoal) (hyp : TSyntax `ident) : OptionT MetaM Expr := do
-  let some decl := (← getLCtx).findFromUserName? hyp.raw.getId | failure
-  OptionT.mk do
+def _root_.MPL.ProofMode.SGoal.exactPure (goal : SGoal) (hyp : TSyntax `term) : TacticM Expr := do
   let T := goal.target
   let expected := mkApp2 (mkConst ``SPred.tautological) goal.σs T
-  unless ← isDefEq decl.type expected do
-    throwError "sexact tactic failed, pure hypothesis {decl.userName} is not definitionally equal to {expected}"
-  return mkApp4 (mkConst ``Exact.from_tautology) goal.σs goal.hyps goal.target (mkFVar decl.fvarId)
+  let prf ← try
+    elabTerm hyp expected
+  catch _ => throwError "sexact tactic failed, {hyp} is not have type {expected}"
+  return mkApp4 (mkConst ``Exact.from_tautology) goal.σs goal.hyps goal.target prf
 
-elab "sexact" colGt hyp:ident : tactic => do
+elab "sexact" colGt hyp:term : tactic => do
   let mvar ← getMainGoal
   mvar.withContext do
   let g ← instantiateMVars <| ← mvar.getType
   let some goal := parseSGoal? g | throwError "not in proof mode"
-  let some proof ← liftMetaM <|
-    goal.exact hyp <|> goal.exactPure hyp
-    | throwError "hypothesis not found"
-  mvar.assign proof
+  if let some prf ← liftMetaM (goal.exact hyp) then
+    mvar.assign prf
+  else
+    mvar.assign (← goal.exactPure hyp)
   replaceMainGoal []
